working zero_array proof

examples/arrays_proofs.v
@@ -1,3 +1,4 @@
+From Coq          Require Import Program.Basics.
 From Coq          Require Import Lists.List.
 From Coq          Require Import String.
 From Coq          Require Import Vectors.Vector.
@@ -12,12 +13,230 @@ Import SAWCorePrelude.
 Require Import Examples.arrays.
 Import arrays.
 
-Lemma no_errors_contains0 : refinesFun contains0 (fun _ _ => noErrorsSpec).
+Import VectorNotations.
+
+Lemma if_bv_lemma (b : bool) : not (bvEq 1 (if b then bvLit 1 1 else bvLit 1 0) (bvLit 1 0)) = b.
 Proof.
-  unfold contains0, contains0__tuple_fun, noErrorsSpec.
+  destruct b; reflexivity.
+Qed.
+
+Definition bvInRange w (x lo hi : SAWCorePrelude.bitvector w) :=
+  and (bvsle w lo x) (bvsle w x hi).
+
+Lemma and_bool_eq_true_lemma (b c : bool) : and b c = true <-> (b = true) /\ (c = true).
+Proof.
+  split.
+  - destruct b, c; auto.
+  - intro; destruct H; destruct b, c; auto.
+Qed.
+
+Lemma and_bool_eq_false_lemma (b c : bool) : and b c = false <-> (b = false) \/ (c = false).
+Proof.
+  split.
+  - destruct b, c; auto.
+  - intro; destruct H; destruct b, c; auto.
+Qed.
+
+Definition isBvsle w a b : Prop := bvsle w a b = true.
+Definition isBvsle_def w a b : bvsle w a b = true <-> isBvsle w a b := reflexivity _.
+Definition isBvsle_def_opp w a b : bvslt w a b = false <-> isBvsle w b a. Admitted.
+Instance PreOrder_isBvsle w : PreOrder (isBvsle w). Admitted.
+
+Definition isBvsle_suc_r w (a : bitvector w) : isBvsle w a (bvAdd w a (bvLit w 1)).
 Admitted.
 
-Lemma no_errors_zero_array : refinesFun zero_array (fun _ _ => noErrorsSpec).
+Definition isBvslt w a b : Prop := bvslt w a b = true.
+Definition isBvslt_def w a b : bvslt w a b = true <-> isBvslt w a b := reflexivity _.
+Definition isBvslt_def_opp w a b : bvsle w a b = false <-> isBvslt w b a. Admitted.
+Instance PreOrder_isBvslt w : PreOrder (isBvslt w). Admitted.
+
+Instance Proper_isBvslt_isBvsle w : Proper (isBvsle w --> isBvsle w ==> impl) (isBvslt w).
+Admitted.
+
+Definition isBvslt_to_isBvsle_suc w a b : isBvslt w a b -> isBvsle w (bvAdd w a (bvLit w 1)) b.
+Admitted.
+
+Definition isBvslt_antirefl w a : ~ isBvslt w a a.
+Admitted.
+
+Definition isBvule w a b : Prop := bvule w a b = true.
+Definition isBvule_def w a b : bvule w a b = true <-> isBvule w a b := reflexivity _.
+Definition isBvule_def_opp w a b : bvult w a b = false <-> isBvule w b a. Admitted.
+Instance PreOrder_isBvule w : PreOrder (isBvule w). Admitted.
+
+Definition isBvult w a b : Prop := bvult w a b = true.
+Definition isBvult_def w a b : bvult w a b = true <-> isBvult w a b := reflexivity _.
+Definition isBvult_def_opp w a b : bvule w a b = false <-> isBvult w b a. Admitted.
+Instance PreOrder_isBvult w : PreOrder (isBvult w). Admitted.
+
+Definition isBvult_to_isBvslt_pos w a b : isBvsle w (bvLit w 0) a ->
+                                          isBvsle w (bvLit w 0) b ->
+                                          isBvult w a b -> isBvslt w a b.
+Admitted.
+
+
+(* Print zero_array__tuple_fun. *)
+
+Definition zero_array_lrt
+  := LRT_Fun (SAWCorePrelude.bitvector 64)
+      (fun arg0 : SAWCorePrelude.bitvector 64 =>
+       LRT_Fun (BVVec 64 arg0 {_ : SAWCorePrelude.bitvector 64 & unit})
+         (fun _ : BVVec 64 arg0 {_ : SAWCorePrelude.bitvector 64 & unit} =>
+          LRT_Ret (BVVec 64 arg0 {_ : SAWCorePrelude.bitvector 64 & unit}))).
+
+Definition zero_array_letRec_lrt
+  := LRT_Fun (SAWCorePrelude.bitvector 64)
+      (fun arg0 : SAWCorePrelude.bitvector 64 =>
+       LRT_Fun (BVVec 64 arg0 {_ : SAWCorePrelude.bitvector 64 & unit})
+         (fun _ : BVVec 64 arg0 {_ : SAWCorePrelude.bitvector 64 & unit} =>
+          LRT_Fun {_ : SAWCorePrelude.bitvector 64 & unit}
+            (fun _ : {_ : SAWCorePrelude.bitvector 64 & unit} =>
+             LRT_Ret (BVVec 64 arg0 {_ : SAWCorePrelude.bitvector 64 & unit})))).
+
+Definition bvMem_lo :=
+  Eval compute in bvLit_0b"1111000000000000000000000000000000000000000000000000000000000000".
+Definition bvMem_hi :=
+  Eval compute in bvLit_0b"0000111111111111111111111111111111111111111111111111111111111111".
+
+Definition zero_array_noErrors : lrtToType zero_array_lrt := fun x _ =>
+  assumingM (bvInRange 64 x (bvLit 64 0) bvMem_hi = true)
+   (letRecM (lrts:=LRT_Cons zero_array_letRec_lrt LRT_Nil)
+            (fun _ => (fun x' _ i => assumingM (bvInRange 64 (projT1 i) (bvLit 64 0) x = true
+                                                /\ x = x')
+                                     noErrorsSpec, tt))
+            (fun _ => noErrorsSpec)).
+
+(* Set Typeclasses Debug. *)
+
+Lemma no_errors_zero_array_manual : refinesFun zero_array zero_array_noErrors.
 Proof.
-  unfold zero_array, zero_array__tuple_fun, noErrorsSpec.
+  unfold zero_array, zero_array__tuple_fun, zero_array_noErrors, noErrorsSpec.
+  unfold zero_array_lrt, zero_array_letRec_lrt.
+  unfold bvultWithProof.
+  (* fold bvMem_lo and bvMem_hi for convenience (Why must I hold Coq's hand so much?? Aghhh!!) *)
+  unfold true, false; fold bvMem_lo; fold bvMem_hi.
+  (* unfold the top-level multiFixM on the left *)
+  apply refinesFun_multiFixM_fst.
+  unfold Datatypes.fst, refinesFun; intros.
+  (* refinesM_assumingM_r, and manipulation of the resulting hyp. *)
+  apply refinesM_assumingM_r; intro e_assuming1.
+  unfold bvInRange in e_assuming1.
+  rewrite and_bool_eq_true_lemma in e_assuming1.
+  repeat rewrite isBvsle_def in e_assuming1.
+  destruct e_assuming1 as [ e_assuming1_H1 e_assuming1_H2 ].
+  (* refinesM_letRecM1_fst *)
+  apply refinesM_letRecM1_fst; try apply ProperFun_any.
+  (* 1. proving refinement of the letRec'd functions *)
+  - (* unfold the multiFixM on the left *)
+    apply refinesFun_multiFixM_fst.
+    unfold Datatypes.fst, refinesFun; intros.
+    (* can we get Coq to do this auomatically too? *)
+    rewrite if_bv_lemma.
+    (* refinesM_assumingM_r, and manipulation of the resulting hyp. *)
+    apply refinesM_assumingM_r; intro e_assuming2; unfold bvInRange in e_assuming2.
+    rewrite and_bool_eq_true_lemma in e_assuming2.
+    destruct e_assuming2 as [ e_assuming2 e_assuming2_H3 ].
+    repeat rewrite isBvsle_def in e_assuming2.
+    destruct e_assuming2 as [ e_assuming2_H1 e_assuming2_H2 ].
+    (* refinesM_if_l, and manipulation of the resulting hyp. *)
+    apply refinesM_if_l; intro e_if1; try rewrite e_if1.
+    + apply refinesM_if_l; intro e_if2.
+      * apply refinesM_maybe_l; [ intro e_maybe | intros e_maybe_arg e_maybe ].
+        -- discriminate e_maybe.
+        -- apply refinesM_assumingM_l.
+           (* I. proving the loop invariant *)
+           ++ unfold bvInRange.
+              rewrite and_bool_eq_true_lemma.
+              split; try split; try rewrite isBvsle_def.
+              ** transitivity (projT1 a3).
+                 --- assumption.
+                 --- apply isBvsle_suc_r.
+              ** apply isBvslt_to_isBvsle_suc.
+                 rewrite isBvult_def in e_if1.
+                 rewrite <- e_assuming2_H3 in e_if1.
+                 apply isBvult_to_isBvslt_pos; assumption.
+              ** assumption.
+           (* II. proving refinement of the bodies *)
+           ++ reflexivity.
+      * (* this case is impossible *)
+        rewrite and_bool_eq_false_lemma in e_if2.
+        destruct e_if2 as [ e_if2 | e_if2 ]; rewrite isBvslt_def_opp in e_if2.
+        -- rewrite <- e_assuming2_H1 in e_if2.
+           vm_compute in e_if2; inversion e_if2.
+        -- rewrite e_assuming2_H2, e_assuming1_H2 in e_if2.
+           apply isBvslt_antirefl in e_if2; inversion e_if2.
+    + prove_refinement.
+  (* 2. proving refinement of the letRec bodies *)
+  - apply refinesM_assumingM_l.
+    (* I. proving the initial loop invariant *)
+    + unfold projT1, bvInRange.
+      rewrite and_bool_eq_true_lemma; split; split.
+      * reflexivity.
+      * assumption.
+    (* II. proving refinement of the bodies *)
+    + reflexivity.
+Qed.
+
+Lemma no_errors_zero_array_auto : refinesFun zero_array zero_array_noErrors.
+Proof.
+  unfold zero_array, zero_array__tuple_fun, zero_array_noErrors, noErrorsSpec.
+  unfold zero_array_lrt, zero_array_letRec_lrt.
+  unfold bvultWithProof.
+  unfold true, false; fold bvMem_lo; fold bvMem_hi.
+  (* apply refinesFun_multiFixM_fst. *)
+  (* unfold Datatypes.fst, refinesFun; intros. *)
+  (* apply refinesM_assumingM_r; intro e_assuming. *)
+  prove_refinement.
+  (* Some hypothesis cleanup used in most of the below cases *)
+  all: try unfold bvInRange in e_assuming, e_assuming0.
+  all: try rewrite and_bool_eq_true_lemma in e_assuming, e_assuming0.
+  all: try repeat rewrite isBvsle_def in e_assuming, e_assuming0.
+  all: try destruct e_assuming  as [ e_assuming_H0 e_assuming_H1 ].
+  all: try destruct e_assuming0 as [ e_assuming0 e_assuming0_H2 ].
+  all: try destruct e_assuming0 as [ e_assuming0_H0 e_assuming0_H1 ].
+  - assumption. (* FIXME Could prove_refinement do this automatically? *)
+  - rewrite if_bv_lemma in e_if.
+    rewrite e_if in e_maybe.
+    discriminate e_maybe.
+  - (* Proving the loop invariant holds inductively: *)
+    simpl; unfold bvInRange.
+    rewrite and_bool_eq_true_lemma.
+    split; try split; try rewrite isBvsle_def.
+    + transitivity (projT1 a3).
+      * assumption.
+      * apply isBvsle_suc_r.
+    + apply isBvslt_to_isBvsle_suc.
+      rewrite if_bv_lemma, isBvult_def in e_if.
+      rewrite <- e_assuming0_H2 in e_if.
+      apply isBvult_to_isBvslt_pos; assumption.
+    + assumption.
+  - assumption. (* FIXME Could prove_refinement do this automatically? *)
+  - (* Proving that this case is absurd, by virtue of out loop invariant: *)
+    rewrite and_bool_eq_false_lemma in e_if0.
+    destruct e_if0 as [ e_if0 | e_if0 ]; rewrite isBvslt_def_opp in e_if0.
+    + rewrite <- e_assuming0_H0 in e_if0.
+      vm_compute in e_if0.
+      inversion e_if0.
+    + rewrite e_assuming0_H1, e_assuming_H1 in e_if0.
+      apply isBvslt_antirefl in e_if0; inversion e_if0.
+  - (* Proving the loop invariant holds initially: *)
+    split.
+    + admit. (* FIXME Hunh?? Is Coq deleting the e_assuming hypothesis...? *)
+    + reflexivity.
+Admitted.
+
+
+Definition contains0_lrt := (LRT_Fun (SAWCorePrelude.bitvector 64)
+                   (fun arg0 : SAWCorePrelude.bitvector 64 =>
+                    LRT_Fun (BVVec 64 arg0 {_ : SAWCorePrelude.bitvector 64 & unit})
+                      (fun _ : BVVec 64 arg0 {_ : SAWCorePrelude.bitvector 64 & unit} =>
+                       LRT_Fun {_ : SAWCorePrelude.bitvector 64 & unit}
+                         (fun _ : {_ : SAWCorePrelude.bitvector 64 & unit} =>
+                          LRT_Ret
+                            (BVVec 64 arg0 {_ : SAWCorePrelude.bitvector 64 & unit} *
+                             ({_ : SAWCorePrelude.bitvector 64 & unit} * unit)))))).
+
+Lemma no_errors_contains0 : refinesFun contains0 (fun _ _ => letRecM (lrts:=LRT_Cons contains0_lrt LRT_Nil) (fun _ => (fun _ _ _ => noErrorsSpec, tt)) (fun _ => noErrorsSpec)).
+Proof.
+  unfold contains0, contains0__tuple_fun, noErrorsSpec.
 Admitted.
